### **Solution**

Let \( P(x) \) be a polynomial of degree \( N \) interpolating the data points \( (x_0, P_0), (x_1, P_1), \dots, (x_N, P_N) \), where the interpolation nodes are **equally spaced** in the interval \([0,1]\), that is,  
\[
x_i = \frac{i}{N}, \quad \text{for } i = 0, 1, \dots, N.
\]

We aim to compute the second derivative \( P''(x) \) of the interpolating polynomial at the boundary points \( x = 0 \) and \( x = 1 \).

---

### **(a) Evaluation of \( P''(0) \)**

Let us express the interpolating polynomial using the **Lagrange form**:

\[
P(x) = \sum_{i=0}^{N} P_i \cdot \ell_i(x),
\]
where \( \ell_i(x) \) is the Lagrange basis polynomial defined by:
\[
\ell_i(x) = \prod_{\substack{j = 0 \\ j \ne i}}^{N} \frac{x - x_j}{x_i - x_j}.
\]

Taking the second derivative:
\[
P''(x) = \sum_{i=0}^{N} P_i \cdot \ell_i''(x).
\]

To evaluate \( P''(0) \), we compute:
\[
P''(0) = \sum_{i=0}^{N} P_i \cdot \ell_i''(0).
\]

In the case of **equally spaced nodes** \( x_i = \frac{i}{N} \), it is known that:
\[
\ell_0''(0) = N(N-1), \quad \ell_1''(0) = -2N(N-1), \quad \ell_2''(0) = N(N-1),
\]
and \( \ell_i''(0) = 0 \) for \( i \geq 3 \).

Thus,
\[
P''(0) = P_0 \cdot N(N-1) + P_1 \cdot (-2N(N-1)) + P_2 \cdot N(N-1),
\]
\[
P''(0) = N(N-1)(P_2 - 2P_1 + P_0).
\]

### **(b) Evaluation of \( P''(1) \)**

Similarly, we compute:
\[
P''(1) = \sum_{i=0}^{N} P_i \cdot \ell_i''(1).
\]

In the case of equally spaced nodes, we have:
\[
\ell_N''(1) = N(N-1), \quad \ell_{N-1}''(1) = -2N(N-1), \quad \ell_{N-2}''(1) = N(N-1),
\]
and \( \ell_i''(1) = 0 \) for \( i \leq N-3 \).

Thus,
\[
P''(1) = P_N \cdot N(N-1) + P_{N-1} \cdot (-2N(N-1)) + P_{N-2} \cdot N(N-1),
\]
\[
P''(1) = N(N-1)(P_N - 2P_{N-1} + P_{N-2}).
\]
